MRiscX/Semantics/Specification.lean
@@ -3,6 +3,8 @@ import MRiscX.Tactics.SpecificationTactics
 import MRiscX.Elab.HoareElaborator
 import MRiscX.Elab.CodeElaborator
 import MRiscX.Delab.DelabHoare
+import Lean
+
 open Lean Elab Tactic
 
 /-
@@ -26,19 +28,25 @@ hold after the execution. The precondition is applied after simulating the
 effects of the instruction.
 -/
 theorem specification_LoadAddress (P: Assertion) (pc addr dst: UInt64) (L: Set UInt64):
+  dst % MRISCX_REG_SIZE.toUInt64 ≠ 0 →
   L = {n : UInt64 | n ≠ pc + 1} →
   hoare
     ⟪la x dst, addr;⟫
     ⦃P ⟦x[dst] ← addr; pc++⟧ ∧ ¬⸨terminated⸩⦄ pc ↦ ⟨{pc+1} | L⟩ ⦃P ⟦⟧ ∧ ¬⸨terminated⸩⦄
   end
   := by
-  intros Hl
+  intros neq_z Hl
   rw [Hl]
   unfold hoare_triple_up_1
   rintro _ _ s HCurr h_pc ⟨pre, h_terminated⟩
   -- rw [pre2] at pre1
   simp at h_terminated
   unfold MState.addRegister at pre
+  simp at pre
+  have: RegisterNr.ofUInt64 dst ≠ 0 := by
+      apply n_not_zero_registerNr_not_zero
+      exact neq_z
+  simp [this] at pre
   unfold weak
   exists s.runOneStep
   apply And.intro
@@ -51,15 +59,15 @@ theorem specification_LoadAddress (P: Assertion) (pc addr dst: UInt64) (L: Set U
         simp [<- MState.run_one_step_eq_run_n_1]
         unfold MState.runOneStep
         rw [h_terminated, ←h_pc, HCurr]
-        simp
+        simp [this]
         zero_lt_ne_zero
   case right =>
       simp [- MState.run_one_step_eq_run_n_1]
       unfold MState.runOneStep MState.getRegisterAt
       rw [HCurr]
-      simp
+      simp [this]
       simp [h_terminated, ←h_pc]
-      simp at pre
+      -- simp at pre
       rw [h_terminated] at pre
       rw [h_pc]
       rw [h_pc] at pre
